Do not deliver to myself

denotational/Network.v
@@ -69,7 +69,11 @@ Module Network(S: SSystem).
     list_replace (h::ts) F1 a := a :: ts;
     list_replace (h::ts) (FS k) a := h :: list_replace ts k a.
 
-  Notation "v '@' i ':=' a" := (list_replace v i a) (at level 70).
+  Equations list_monomap_except{A}(f: A -> A)(l: list A)(i: fin (length l)): list A :=
+    list_monomap_except f (h::ts) F1 := h :: map f ts;
+    list_monomap_except f (h::ts) (FS k) := f h :: list_monomap_except f ts k.
+    
+  Notation "v '@' i ':=' a" := (list_replace v i a) (at level 80).
   Notation "v '$' i" := (safe_nth v i) (at level 80).
   Notation "v '--' i" := (list_rm v i) (at level 80).
   
@@ -88,6 +92,20 @@ Module Network(S: SSystem).
             cbn; auto.
   Defined.
 
+  Lemma list_monomap_except_length_eq:
+    forall A (v: list A)(f: A -> A) i,
+      length (list_monomap_except f v i) = length v.
+  Proof.
+    dependent induction v; cbn; intros.
+    - inversion i.
+    - dependent destruction i.
+      + replace (list_monomap_except f (a :: v) (@F1 (length v)))
+          with (a :: map f v) by reflexivity; cbn;
+          rewrite map_length; reflexivity.
+      + replace (list_monomap_except f (a :: v) (FS i))
+          with (f a :: list_monomap_except f v i) by reflexivity; cbn; auto.
+  Defined.
+        
   (** TODO: figure out UID <-> fin t mapping *)
   Parameter uid_to_fin: forall t, uid -> fin t.
   Parameter fin_to_uid: forall t, fin t -> uid.
@@ -142,11 +160,12 @@ Module Network(S: SSystem).
       | VisF (Broadcast b) k =>
           (** TODO: Make non-det on each agent *)
           let msg := {| principal := fin_to_uid i; payload := b |} in
-          let sys' := map (fun a: list Msg * itree Net R =>
-                             let (q, a') := a in (msg :: q, a')
-                          ) sys in
+          (** Does not deliver msg back to sender *)
+          let sys' := list_monomap_except
+                        (fun a: list Msg * itree Net R =>
+                           let (q, a') := a in (msg :: q, a')) sys i in
           let i' := eq_rec_r (fun n: nat => fin n) i
-                             (map_length _ sys) in
+                             (list_monomap_except_length_eq _ sys _ i) in
           CTrees.TauV (schedule (sys' @ i' := (q, k tt)) done)
 
       end.
